% --------------------------------------------------------------
% This is all preamble stuff that you don't have to worry about.
% Head down to where it says "Start here"
% --------------------------------------------------------------
 
\documentclass[12pt]{article}
 
\usepackage[margin=1in]{geometry} 
\usepackage{amsmath,amsthm,amssymb}
\usepackage{enumitem}
\usepackage{graphicx}
\usepackage{indentfirst}
\usepackage{tikz, tkz-euclide}
\usepackage{float}
\usepackage{changepage}
\usepackage{titling}
\usepackage{wrapfig}
\usetikzlibrary{calc}
\usetikzlibrary{positioning}
\graphicspath{ {./images/} }
 
\newcommand{\N}{\mathbb{N}}
\newcommand{\Z}{\mathbb{Z}}
\newcommand{\R}{\mathbb{R}}
\DeclareMathOperator{\arctantwo}{arctan2}


\setlength{\parindent}{10pt}
\interfootnotelinepenalty=10000
\setlength{\footskip}{15pt}

 
\newenvironment{theorem}[2][Theorem]{\begin{trivlist}
\item[\hskip \labelsep {\bfseries #1}\hskip \labelsep {\bfseries #2.}]}{\end{trivlist}}
\newenvironment{lemma}[2][Lemma]{\begin{trivlist}
\item[\hskip \labelsep {\bfseries #1}\hskip \labelsep {\bfseries #2.}]}{\end{trivlist}}
\newenvironment{exercise}[2][Exercise]{\begin{trivlist}
\item[\hskip \labelsep {\bfseries #1}\hskip \labelsep {\bfseries #2.}]}{\end{trivlist}}
\newenvironment{problem}[2][Problem]{\begin{trivlist}
\item[\hskip \labelsep {\bfseries #1}\hskip \labelsep {\bfseries #2.}]}{\end{trivlist}}
\newenvironment{question}[2][Question]{\begin{trivlist}
\item[\hskip \labelsep {\bfseries #1}\hskip \labelsep {\bfseries #2.}]}{\end{trivlist}}
\newenvironment{corollary}[2][Corollary]{\begin{trivlist}
\item[\hskip \labelsep {\bfseries #1}\hskip \labelsep {\bfseries #2.}]}{\end{trivlist}}
 
\begin{document}
 
% --------------------------------------------------------------
%                         Start here
% --------------------------------------------------------------

\setlength{\droptitle}{0pt}
\title{Week3\_ECON\_PS1}%replace X with the appropriate %number
\author{\vspace{0pt} Shiqi Li}%if necessary, replace with your %course title
\date{}
 
\maketitle
 
\textbf{Exercise 1} \par
    
    \begin{align*}
        \frac{1}{e^{z_{t}} K_{t}^{\alpha}-K_{t+1}} &= \beta E_{t}\left\{\frac{\alpha e^{z_{t+1}} K_{t+1}^{\alpha-1}}{e^{z_{t+1}} K_{t+1}^{\alpha}-K_{t+2}}\right\} \\
        \intertext{Sub in the guessed policy function and $z_t = 0$ we get}
        \frac{1}{K_{t}^{\alpha}-A K_{t}^\alpha} &= \beta \left\{\frac{\alpha (A {K_{t}}^\alpha)^{\alpha-1}}{{(A {K_t}^\alpha)}^{\alpha}- {A(A {K_t}^\alpha)}^{\alpha}}\right\} \\
        1 &= \frac{\beta}{A} \left\{\frac{\alpha (A {K_{t}}^\alpha)^{\alpha-1}}{{(A {K_t}^\alpha)}^{\alpha-1}- {(A {K_t}^\alpha)}^{\alpha-1}}\right\} \\
        1 &= \frac{\alpha \beta}{A}\\
        A &= \alpha \beta\\
        \intertext{So $\overline{K}$ is:}
        \overline{K} &= (\alpha \beta)^{\frac{1}{1-\alpha}}
        \intertext{Check for steady state policy function, if $K_t$ is a steady state, then}
        K_{t+1} = (\alpha \beta)\left[(\alpha \beta)^{\frac{1}{1-\alpha}}\right]^{\alpha} &= (\alpha \beta)^{\frac{1}{1-\alpha}} = K_{t}
    \end{align*}
        
\textbf{Exercise 2} \par
    Characterizing functions:
    \begin{gather}
        c_{t}=(1-\tau)\left[w_{t} \ell_{t}+\left(r_{t}-\delta\right) k_{t}\right]+k_{t}+T_{t}-k_{t+1} \\
        \frac{1}{c_{t}}=\beta E_{t}\left\{\frac{1}{c_{t+1}}\left[\left(r_{t+1}-\delta\right)(1-\tau)+1\right]\right\} \\
        \frac{\alpha}{1-\ell_t}=\frac{1}{c_{t}} w_{t}(1-\tau) \\
        r_{t}=\alpha e^{z_{t}} K_{t}^{\alpha - 1} L_{t}^{1-\alpha} \\
        w_{t}=(1-\alpha) e^{z_{t}} K_{t}^{\alpha} L_{t}^{-\alpha} \\
        \tau\left[w_{t} \ell_{t}+\left(r_{t}-\delta\right) k_{t}\right]=T_{t} \\
        z_{t}=\left(1-\rho_{z}\right) \overline{z}+\rho_{z} z_{t-1}+\epsilon_{t}^{z} ; \quad \epsilon_{t}^{z} \sim \text { i.i.d. }\left(0, \sigma_{z}^{2}\right)
    \end{gather}

\textbf{Exercise 3} \par
    Characterizing functions:
    \begin{gather}
        c_{t}=(1-\tau)\left[w_{t} \ell_{t}+\left(r_{t}-\delta\right) k_{t}\right]+k_{t}+T_{t}-k_{t+1} \\
        {c_{t}}^{-\gamma}=\beta E_{t}\left\{{c_{t+1}}^{-\gamma}\left[\left(r_{t+1}-\delta\right)(1-\tau)+1\right]\right\} \\
        \frac{\alpha}{1-\ell_t}={c_{t}}^{-\gamma} w_{t}(1-\tau) \\
        r_{t}=\alpha e^{z_{t}} K_{t}^{\alpha - 1} L_{t}^{1-\alpha} \\
        w_{t}=(1-\alpha) e^{z_{t}} K_{t}^{\alpha} L_{t}^{-\alpha} \\
        \tau\left[w_{t} \ell_{t}+\left(r_{t}-\delta\right) k_{t}\right]=T_{t} \\
        z_{t}=\left(1-\rho_{z}\right) \overline{z}+\rho_{z} z_{t-1}+\epsilon_{t}^{z} ; \quad \epsilon_{t}^{z} \sim \text { i.i.d. }\left(0, \sigma_{z}^{2}\right)
    \end{gather}
    
\textbf{Exercise 4} \par
    Characterizing functions:
    \begin{gather}
        c_{t}=(1-\tau)\left[w_{t} \ell_{t}+\left(r_{t}-\delta\right) k_{t}\right]+k_{t}+T_{t}-k_{t+1} \\
        {c_{t}}^{-\gamma}=\beta E_{t}\left\{{c_{t+1}}^{-\gamma}\left[\left(r_{t+1}-\delta\right)(1-\tau)+1\right]\right\} \\
        -\alpha (1-\ell_t)^{-\epsilon}={c_{t}}^{-\gamma} w_{t}(1-\tau) \\
        r_{t}=\alpha e^{z_{t}} K_{t}^{\eta - 1} \left[\alpha K_{t}^{\eta}+(1-\alpha) L_{t}^{\eta}\right]^{\frac{1 - \eta}{\eta}} \\
        w_{t}=(1-\alpha) e^{z_{t}} L_{t}^{\eta - 1} \left[ \alpha K_{t}^{\eta}+(1-\alpha) L_{t}^{\eta}\right]^{\frac{1 - \eta}{\eta}} \\
        \tau\left[w_{t} \ell_{t}+\left(r_{t}-\delta\right) k_{t}\right]=T_{t} \\
        z_{t}=\left(1-\rho_{z}\right) \overline{z}+\rho_{z} z_{t-1}+\epsilon_{t}^{z} ; \quad \epsilon_{t}^{z} \sim \text { i.i.d. }\left(0, \sigma_{z}^{2}\right)
    \end{gather}
    
\textbf{Exercise 5} \par
    Characterizing functions:
    \begin{gather}
        c_{t}=(1-\tau)\left[w_{t}+\left(r_{t}-\delta\right) k_{t}\right]+k_{t}+T_{t}-k_{t+1} \\
        {c_{t}}^{-\gamma}=\beta E_{t}\left\{{c_{t+1}}^{-\gamma}\left[\left(r_{t+1}-\delta\right)(1-\tau)+1\right]\right\} \\
        0={c_{t}}^{-\gamma} w_{t}(1-\tau) \\
        r_{t}=\alpha e^{z_{t}} K_{t}^{\alpha - 1} L_{t}^{1-\alpha} \\
        w_{t}=(1-\alpha) {e^{z_{t}}}^{(1-\alpha)} K_{t}^{\alpha} L_{t}^{-\alpha} \\
        \tau\left[w_{t}+\left(r_{t}-\delta\right) k_{t}\right]=T_{t} \\
        z_{t}=\left(1-\rho_{z}\right) \overline{z}+\rho_{z} z_{t-1}+\epsilon_{t}^{z} ; \quad \epsilon_{t}^{z} \sim \text { i.i.d. }\left(0, \sigma_{z}^{2}\right)
    \end{gather}
    Steady state versions:
    \begin{gather}
        c=(1-\tau)\left[w+\left(r-\delta\right) k\right]+T \\
        {c}^{-\gamma}=\beta \left\{{c}^{-\gamma}\left[\left(r-\delta\right)(1-\tau)+1\right]\right\} \\
        0={c}^{-\gamma} w(1-\tau) \\
        r=\alpha k^{\alpha - 1} \\
        w=(1-\alpha) k^{\alpha} \\
        \tau\left[w+\left(r-\delta\right) k\right]=T
    \end{gather}
    Algebraic solusion:
    
\textbf{Exercise 6} \par
    Characterizing functions:
    \begin{gather}
        c_{t}=(1-\tau)\left[w_{t} \ell_{t}+\left(r_{t}-\delta\right) k_{t}\right]+k_{t}+T_{t}-k_{t+1} \\
        {c_{t}}^{-\gamma}=\beta E_{t}\left\{{c_{t+1}}^{-\gamma}\left[\left(r_{t+1}-\delta\right)(1-\tau)+1\right]\right\} \\
        -a (1-\ell_t)^{-\epsilon}={c_{t}}^{-\gamma} w_{t}(1-\tau) \\
        r_{t}=\alpha e^{z_{t}} K_{t}^{\alpha - 1} L_{t}^{1-\alpha} \\
        w_{t}=(1-\alpha) {e^{z_{t}}}^{(1-\alpha)} K_{t}^{\alpha} L_{t}^{-\alpha} \\
        \tau\left[w_{t}+\left(r_{t}-\delta\right) k_{t}\right]=T_{t} \\
        z_{t}=\left(1-\rho_{z}\right) \overline{z}+\rho_{z} z_{t-1}+\epsilon_{t}^{z} ; \quad \epsilon_{t}^{z} \sim \text { i.i.d. }\left(0, \sigma_{z}^{2}\right)
    \end{gather}
    Steady state versions:
    \begin{gather}
        c=(1-\tau)\left[w \ell+\left(r-\delta\right) k\right]+T \\
        {c}^{-\gamma}=\beta {c}^{-\gamma}\left[\left(r-\delta\right)(1-\tau)+1\right] \\
        -a (1-\ell_t)^{-\epsilon} = {c}^{-\gamma} w(1-\tau) \\
        r=\alpha k^{\alpha - 1} \ell^{1-\alpha}\\
        w=(1-\alpha) k^{\alpha} \ell^{-\alpha}\\
        \tau\left[w+\left(r-\delta\right) k\right]=T
    \end{gather}
 
% --------------------------------------------------------------
%     You don't have to mess with anything below this line.
% --------------------------------------------------------------
 
\end{document}
